refactor in poly, add implicit pass for constructors

src/theories/PolyFirstOrder.v
@@ -8,47 +8,50 @@ Set Universe Polymorphism.
 
 Section PolySyntax.
 
-(* Definition ty_ctx := snoc_list Type. *)
 Definition ty_ctx := nat.
-Context (sig_sorts : nat -> Type).
+Context {sig_sorts : nat -> Type}.
 
 Inductive ty_valu {T: Type} : ty_ctx -> snoc_list T -> Type := 
 | TVEmp : 
   ty_valu 0 SLNil
 | TVSnoc : 
-  forall ctx t sl, 
+  forall {ctx sl}, 
     ty_valu ctx sl -> 
-    ty_valu (S ctx) (Snoc sl t).
+    forall t, 
+      ty_valu (S ctx) (Snoc sl t).
 
 Inductive ty_ctx_var: ty_ctx -> Type :=
 | TCVHere:
-  forall ctx,
+  forall {ctx},
     ty_ctx_var (S ctx)
 | TCVThere:
-  forall ctx,
+  forall {ctx},
     ty_ctx_var ctx ->
     ty_ctx_var (S ctx).
 
 Inductive ty_expr_var : ty_ctx -> nat -> Type := 
 | TEVAnon  : 
-  forall ctx,
+  forall {ctx},
     ty_ctx_var ctx -> 
     ty_expr_var ctx 0
 | TEVNamed : 
-  forall ctx arity, 
+  forall {ctx arity}, 
     sig_sorts arity ->  
     ty_expr_var ctx arity.
 
 Inductive ty_expr (ctx: ty_ctx) : nat -> Type := 
 | TEVar : 
-  forall arity, 
+  forall {arity}, 
     ty_expr_var ctx arity -> 
     ty_expr ctx arity
 | TEApp : 
-  forall arity, (* apply a type function *)
+  forall {arity}, (* apply a type function *)
     ty_expr ctx (S arity) -> 
     ty_expr ctx 0 -> 
     ty_expr ctx arity.
+
+Arguments TEVar {_ _} _.
+Arguments TEApp {_ _} _ _.
 
 Record signature: Type :=
   { sig_funs: forall ctx, list (ty_expr ctx 0) -> ty_expr ctx 0 -> Type;
@@ -56,17 +59,17 @@ Record signature: Type :=
 
 Definition ctx t_ctx := snoc_list (ty_expr t_ctx 0).
 
-Inductive var: forall t_ctx, ctx t_ctx -> ty_expr t_ctx 0 -> Type := 
+Inductive var: forall {t_ctx}, ctx t_ctx -> ty_expr t_ctx 0 -> Type := 
 | VHere:
-  forall t_ctx (c: ctx t_ctx) e,
-    var t_ctx (Snoc c e) e
+  forall {t_ctx} {c: ctx t_ctx} {e},
+    var (Snoc c e) e
 | VThere:
-  forall t_ctx (c: ctx t_ctx) s s',
-    var t_ctx c s' ->
-    var _ (Snoc c s) s'.
+  forall {t_ctx} {c: ctx t_ctx} {s s'},
+    var c s' ->
+    var (Snoc c s) s'.
 Derive Signature NoConfusion for var.
 
-Context (sig: signature).
+Context {sig: signature}.
 
 
 (* A list of type expressions in an outer context, with same size as an inner context.
@@ -77,9 +80,8 @@ Context (sig: signature).
 Definition ty_params t_ctx_outer := @ty_valu (ty_expr t_ctx_outer 0).
 
 Equations lookup_tp_var t_ctx_outer t_ctx_inner tys (tp: ty_params t_ctx_outer t_ctx_inner tys) (tc_var: ty_ctx_var t_ctx_inner) : ty_expr t_ctx_outer 0 := {
-  lookup_tp_var _ _ _ (TVSnoc _ e _ _) (TCVHere _) := 
-    e; 
-  lookup_tp_var _ _ _ (TVSnoc _ _ _ tv') (TCVThere _ tc_var') := 
+  lookup_tp_var _ _ _ (TVSnoc _ e) TCVHere := e; 
+  lookup_tp_var _ _ _ (TVSnoc tv' _) (TCVThere tc_var') := 
     lookup_tp_var _ _ _ tv' tc_var'; 
 }.
 
@@ -88,76 +90,78 @@ Equations apply_ty_args
   t_ctx_inner t_ctx_outer t_args n
   (ty_args: ty_params t_ctx_outer t_ctx_inner t_args)
   (te_inner : ty_expr t_ctx_inner n) : ty_expr t_ctx_outer n by struct te_inner := {
-  apply_ty_args _ t_ctx_outer _ _ tp (TEApp _ _ l r) := 
-    TEApp _ _ (apply_ty_args _ _ _ _ _ l) (apply_ty_args _ _ _ _ _ r);
-  apply_ty_args _ _ _ _ tp (TEVar _ _ (TEVNamed _ _ f)) := 
-    TEVar _ _ (TEVNamed _ _ f);
-  apply_ty_args _ _ _ _ tp (TEVar _ _ (TEVAnon _ v)) := 
+  apply_ty_args _ t_ctx_outer _ _ tp (TEApp l r) := 
+    TEApp (apply_ty_args _ _ _ _ _ l) (apply_ty_args _ _ _ _ _ r);
+  apply_ty_args _ _ _ _ tp (TEVar (TEVNamed f)) := 
+    TEVar (TEVNamed f);
+  apply_ty_args _ _ _ _ tp (TEVar (TEVAnon v)) := 
     lookup_tp_var _ _ _ tp v;
 }.
 
-Inductive tm t_ctx : ctx t_ctx -> ty_expr t_ctx 0 -> Type :=
+Inductive tm {t_ctx} : ctx t_ctx -> ty_expr t_ctx 0 -> Type :=
 | TVar: 
-  forall c s,
-    var t_ctx c s ->
-    tm t_ctx c s
+  forall {c s},
+    var c s ->
+    tm c s
 | TFun:
-  forall t_ctx' t_args c args ret,
+  forall {t_ctx' args ret} {t_args} {c: ctx t_ctx},
     sig.(sig_funs) t_ctx' args ret ->
     forall (ty_args : ty_params t_ctx t_ctx' t_args), (* type arguments *)
-      HList.t (tm t_ctx c) (List.map (apply_ty_args t_ctx' t_ctx t_args 0 ty_args) args) -> 
-      tm t_ctx c (apply_ty_args t_ctx' t_ctx t_args 0 ty_args ret). 
+      HList.t (tm c) (List.map (apply_ty_args t_ctx' t_ctx t_args 0 ty_args) args) -> 
+      tm c (apply_ty_args t_ctx' t_ctx t_args 0 ty_args ret). 
 
 Derive Signature for tm.
 
-Inductive fm t_ctx : ctx t_ctx -> Type :=
+Inductive fm {t_ctx} : ctx t_ctx -> Type :=
 (* True and False *)
-| FTrue: forall c, fm t_ctx c
-| FFalse: forall c, fm t_ctx c
+| FTrue: forall {c}, fm c
+| FFalse: forall {c}, fm c
 (* Equality *)
 | FEq: 
-  forall c s,
-    tm t_ctx c s ->
-    tm t_ctx c s ->
-    fm t_ctx c
+  forall {c s},
+    tm c s ->
+    tm c s ->
+    fm c
 (* A relation (with arguments) *)
 | FRel:
-  forall t_ctx' t_args c args,
+  forall {t_ctx' args} {t_args} {c: ctx t_ctx},
     sig.(sig_rels) t_ctx' args ->
     forall (ty_args : ty_params t_ctx t_ctx' t_args), (* type arguments *)
-      HList.t (tm t_ctx c) (List.map (apply_ty_args t_ctx' t_ctx t_args 0 ty_args) args) -> 
-      fm t_ctx c 
+      HList.t (tm c) (List.map (apply_ty_args t_ctx' t_ctx t_args 0 ty_args) args) -> 
+      fm c
 (* Negation, disjunction, conjunction, and implication *)
-| FNeg: forall c, fm t_ctx c -> fm t_ctx c
-| FOr: forall c, fm t_ctx c -> fm t_ctx c -> fm t_ctx c
-| FAnd: forall c, fm t_ctx c -> fm t_ctx c -> fm t_ctx c
-| FImpl: forall c, fm t_ctx c -> fm t_ctx c -> fm t_ctx c
-| FBiImpl: forall c, fm t_ctx c -> fm t_ctx c -> fm t_ctx c
+| FNeg: forall {c}, fm c -> fm c
+| FOr: forall {c}, fm c -> fm c -> fm c
+| FAnd: forall {c}, fm c -> fm c -> fm c
+| FImpl: forall {c}, fm c -> fm c -> fm c
+| FBiImpl: forall {c}, fm c -> fm c -> fm c
 (* Quantification *)
 | FForall:
-  forall c s,
-    fm t_ctx (Snoc c s) ->
-    fm t_ctx c
+  forall {c} s,
+    fm (Snoc c s) ->
+    fm c
 | FExists:
-  forall c s,
-    fm t_ctx (Snoc c s) ->
-    fm t_ctx c.
+  forall {c} s,
+    fm (Snoc c s) ->
+    fm c.
 Derive Signature for fm.
 
 Inductive poly_fm : ty_ctx -> Type := 
 | PFm : 
-  forall tc, 
-    fm tc SLNil -> 
+  forall {tc}, 
+    fm (SLNil : ctx tc)  -> 
     poly_fm tc
 | PForall : 
-  forall tc, 
+  forall {tc}, 
     poly_fm (S tc) -> 
     poly_fm tc.
 End PolySyntax.
 
-Section PolySemantics.
 
-Context (sig_sorts : nat -> Type).
+Arguments TEVar {_ _ _} _.
+Arguments TEApp {_ _ _} _ _.
+
+Section PolySemantics.
 
 Fixpoint arity_ftor (n: nat) : Type := 
   match n with 
@@ -165,49 +169,49 @@ Fixpoint arity_ftor (n: nat) : Type :=
   | (S n) => (Type -> arity_ftor n)
   end.
 
-Context `(interp_sorts : forall n, sig_sorts n -> arity_ftor n).
-
-Context `(sig: signature sig_sorts).
+Context {sig_sorts : nat -> Type}.
+Context {interp_sorts : forall n, sig_sorts n -> arity_ftor n}.
+Context {sig: @signature sig_sorts}.
 
 Set Transparent Obligations.
 
 Equations lookup_tc_var {A} ctx (tys: snoc_list A) (tv: ty_valu ctx tys) (tc_var: ty_ctx_var ctx) : A := {
-  lookup_tc_var _ _ (TVSnoc _ T _ _) (TCVHere _) := T; 
-  lookup_tc_var _ _ (TVSnoc _ _ _ tv') (TCVThere _ tc_var') := lookup_tc_var _ _ tv' tc_var'; 
+  lookup_tc_var _ _ (TVSnoc _ T) TCVHere := T; 
+  lookup_tc_var _ _ (TVSnoc tv' _) (TCVThere tc_var') := lookup_tc_var _ _ tv' tc_var'; 
 }.
 
-Equations interp_te_var ctx (tys: snoc_list Type) (tv: ty_valu ctx tys) n (te_var: ty_expr_var sig_sorts ctx n) : arity_ftor n := {
-  interp_te_var _ _ tv _ (TEVAnon _ v) := 
+Equations interp_te_var ctx (tys: snoc_list Type) (tv: ty_valu ctx tys) n (te_var: @ty_expr_var sig_sorts ctx n) : arity_ftor n := {
+  interp_te_var _ _ tv _ (TEVAnon v) := 
     lookup_tc_var _ _ tv v;
-  interp_te_var ctx _ _ n (TEVNamed _ _ f) := 
+  interp_te_var ctx _ _ n (TEVNamed f) := 
     interp_sorts _ f;
 }.
 
-Equations interp_te ctx (tys: snoc_list Type) (tv: ty_valu ctx tys) n (te: ty_expr sig_sorts ctx n) : arity_ftor n := {
-  interp_te _ _ tv n (TEVar _ v) := 
+Equations interp_te ctx (tys: snoc_list Type) (tv: ty_valu ctx tys) n (te: @ty_expr sig_sorts ctx n) : arity_ftor n := {
+  interp_te _ _ tv n (TEVar v) := 
     interp_te_var _ _ tv n v;
-  interp_te ctx tys tv _ (TEApp _ l r) := 
+  interp_te ctx tys tv _ (TEApp l r) := 
     let T := interp_te ctx tys tv _ r in 
       (interp_te ctx tys tv _ l) T;
 }.
 
 Equations apply_outer_params_tv
   t_ctx_inner t_ctx_outer t_args (tys_outer: snoc_list Type)
-  (ty_args: ty_params sig_sorts t_ctx_outer t_ctx_inner t_args)
+  (ty_args: @ty_params sig_sorts t_ctx_outer t_ctx_inner t_args)
   (tv_outer : ty_valu t_ctx_outer tys_outer) 
   : ty_valu t_ctx_inner (sl_map (interp_te _ _ tv_outer 0) t_args) 
     by struct ty_args := {
   apply_outer_params_tv _ _ _ _ TVEmp _ := TVEmp;
-  apply_outer_params_tv _ _ _ _ (TVSnoc _ e _ tp') _ := TVSnoc _ _ _ (apply_outer_params_tv _ _ _ _ tp' _);
+  apply_outer_params_tv _ _ _ _ (TVSnoc tp' _) _ := TVSnoc (apply_outer_params_tv _ _ _ _ tp' _) _;
 }.
 
 Local Obligation Tactic := intros.
 Equations lookup_tvar_apply_eq {ctx t_ctx tys t_args tv} tp tvar :
-  interp_te t_ctx tys tv 0 (lookup_tp_var sig_sorts t_ctx ctx t_args tp tvar) =
+  interp_te t_ctx tys tv 0 (@lookup_tp_var sig_sorts t_ctx ctx t_args tp tvar) =
   lookup_tc_var ctx (sl_map (interp_te t_ctx tys tv 0) t_args) (apply_outer_params_tv ctx t_ctx t_args tys tp tv) tvar
   by struct tvar := {
-  lookup_tvar_apply_eq (TVSnoc _ _ _ _) (TCVHere _) := eq_refl;
-  lookup_tvar_apply_eq (TVSnoc _ _ _ _) (TCVThere _ _) := _;
+  lookup_tvar_apply_eq (TVSnoc _ _) TCVHere := eq_refl;
+  lookup_tvar_apply_eq (TVSnoc _ _) (TCVThere _) := _;
 }.
 Next Obligation.
   autorewrite with lookup_tp_var.
@@ -221,7 +225,7 @@ Local Obligation Tactic := (unfold RelationClasses.complement, Equivalence.equiv
 
 Lemma apply_outer_eq:
   forall n t_ctx t_ctx' tys t_args tp tv e, 
-    interp_te t_ctx tys tv n (apply_ty_args sig_sorts t_ctx' t_ctx t_args n tp e) 
+    interp_te t_ctx tys tv n (@apply_ty_args sig_sorts t_ctx' t_ctx t_args n tp e) 
     = 
     interp_te t_ctx' (sl_map (interp_te t_ctx tys tv 0) t_args) (apply_outer_params_tv t_ctx' t_ctx t_args tys tp tv) n e.
 Proof.
@@ -244,51 +248,52 @@ induction e.
 Defined.
 
 
-Record interp_sig (sig: signature sig_sorts) := {
+Record interp_sig (sig: @signature sig_sorts) := {
   interp_funs: 
     forall t_ctx ctx args ret, 
-      sig_funs sig_sorts sig t_ctx args ret -> 
+      sig_funs sig t_ctx args ret -> 
       forall (tv: ty_valu t_ctx ctx), 
         HList.t (interp_te t_ctx ctx tv 0) args ->
         interp_te t_ctx ctx tv 0 ret;
   interp_rels: 
     forall t_ctx ctx args, 
-      sig_rels sig_sorts sig t_ctx args -> 
+      sig_rels sig t_ctx args -> 
       forall (tv: ty_valu t_ctx ctx), 
         HList.t (interp_te t_ctx ctx tv 0) args ->
         Prop;
 }.
 
-Context (model: interp_sig sig).
+Context {model: interp_sig sig}.
 
-Inductive valu ty_ctx tys (tv: ty_valu ty_ctx tys) : ctx sig_sorts ty_ctx -> Type := 
+Inductive valu {ty_ctx tys} (tv: ty_valu ty_ctx tys) : @ctx sig_sorts ty_ctx -> Type := 
 | VEmp : 
-  valu ty_ctx tys tv SLNil
+  valu tv SLNil
 | VSnoc : 
-  forall sl e, 
-    valu ty_ctx tys tv sl -> 
+  forall {sl e}, 
+    valu tv sl -> 
     interp_te ty_ctx tys tv 0 e ->
-    valu ty_ctx tys tv (Snoc sl e).
+    valu tv (Snoc sl e).
 
-Equations interp_var t_ctx tys tv e_ctx e (env: valu t_ctx tys tv e_ctx) (v: var sig_sorts _ e_ctx e) : interp_te t_ctx tys tv 0 e := {
-  interp_var _ _ _ _ _ (VSnoc _ _ _ v) (VHere _ _ _ ) := v;
-  interp_var _ _ _ _ _ (VSnoc _ _ env _) (VThere _ _ _ _ vi) := interp_var _ _ _ _ _ env vi;
+Arguments VEmp {_ _ _}.
+Arguments VSnoc {_ _ _ _ _} _ _.
+
+Equations interp_var t_ctx tys (tv: ty_valu t_ctx tys) e_ctx e (env: valu tv e_ctx) (v: var e_ctx e) : interp_te t_ctx tys tv 0 e := {
+  interp_var _ _ _ _ _ (VSnoc _ v) VHere := v;
+  interp_var _ _ _ _ _ (VSnoc env _) (VThere vi) := interp_var _ _ _ _ _ env vi;
 }.
 
-Set Transparent Obligations.
-(* Obligation Tactic := intros. *)
 Equations 
   interp_tm 
-    t_ctx tys tv e_ctx e 
-    (env: valu t_ctx tys tv e_ctx) 
-    (t: tm sig_sorts sig t_ctx e_ctx e) 
+    t_ctx tys (tv: ty_valu t_ctx tys) e_ctx e 
+    (env: valu tv e_ctx) 
+    (t: tm (sig := sig) e_ctx e) 
   : interp_te t_ctx tys tv 0 e 
     by struct t 
   := {
-  interp_tm _ _ _ _ _ env (TVar _ _ v) := 
+  interp_tm _ _ _ _ _ env (TVar v) := 
     interp_var _ _ _ _ _ env v;
-  interp_tm _ tys tv _ _ env (TFun _ t_args _ _ _ f tp hargs) :=
-    let inner := interp_tms _ _ tv _ env _ hargs in
+  interp_tm _ tys tv _ _ env (@TFun _ _ _ t_args _ f tp hargs) :=
+    let inner := interp_tms _ _ tv _ _ env hargs in
     let swapped := HList.map_swap _ _ inner in 
     let trans_args := HList.map _ swapped in 
     let inner_v := 
@@ -298,11 +303,10 @@ Equations
       (* _; *)
 } where 
   interp_tms 
-    t_ctx ctx tv e_ctx 
-    (env: valu t_ctx ctx tv e_ctx) tys 
+    t_ctx ctx (tv: ty_valu t_ctx ctx) e_ctx tys
+    (env: valu tv e_ctx)  
     (tms: HList.t 
-      (fun (te : ty_expr sig_sorts t_ctx 0) => 
-        tm sig_sorts sig t_ctx e_ctx te) 
+      (fun (te : ty_expr t_ctx 0) => tm (sig := sig) e_ctx te) 
       tys
     ) 
   : HList.t (interp_te t_ctx ctx tv 0) tys by struct tms := {
@@ -316,378 +320,48 @@ erewrite apply_outer_eq in X.
 apply X.
 Defined.
 
-Equations interp_fm t_ctx tys tv e_ctx (env: valu t_ctx tys tv e_ctx) (f: fm sig_sorts sig t_ctx e_ctx) : Prop := {
-  interp_fm _ _ _ _ _ (FTrue _) := True;
-  interp_fm _ _ _ _ _ (FFalse _) := False;
-  interp_fm _ _ _ _ _ (FEq _ _ l r) := 
+Equations interp_fm t_ctx tys (tv: ty_valu t_ctx tys) e_ctx (env: valu tv e_ctx) (f: fm (sig := sig) e_ctx) : Prop := {
+  interp_fm _ _ _ _ _ FTrue := True;
+  interp_fm _ _ _ _ _ FFalse := False;
+  interp_fm _ _ _ _ _ (FEq l r) := 
     (interp_tm _ _ _ _ _ _ l) = (interp_tm _ _ _ _ _ _ r);
-  interp_fm _ _ tv _ env (FRel _ t_args _ _ f tp hargs) :=
-    let inner := interp_tms _ _ tv _ env _ hargs in
+  interp_fm _ _ tv _ env (@FRel _ _ t_args _ f tp hargs) :=
+    let inner := interp_tms _ _ tv _ _ env hargs in
     let swapped := HList.map_swap _ _ inner in 
     let trans_args := HList.map _ swapped in 
       model.(interp_rels sig) _ (sl_map (interp_te _ _ tv 0) t_args) _ f (apply_outer_params_tv _ _ _ _ tp tv) trans_args;
-  interp_fm _ _ _ _ _ (FAnd _ l r) := 
+  interp_fm _ _ _ _ _ (FAnd l r) := 
     interp_fm _ _ _ _ _ l /\ interp_fm _ _ _ _ _ r ;
-  interp_fm _ _ _ _ _ (FOr _ l r) := 
+  interp_fm _ _ _ _ _ (FOr l r) := 
     interp_fm _ _ _ _ _ l \/ interp_fm _ _ _ _ _ r ;
-  interp_fm _ _ _ _ _ (FImpl _ l r) := 
+  interp_fm _ _ _ _ _ (FImpl l r) := 
     interp_fm _ _ _ _ _ l -> interp_fm _ _ _ _ _ r ;
-  interp_fm _ _ _ _ _ (FBiImpl _ l r) := 
+  interp_fm _ _ _ _ _ (FBiImpl l r) := 
     interp_fm _ _ _ _ _ l <-> interp_fm _ _ _ _ _ r ;
-  interp_fm _ _ _ _ _ (FNeg _ f) := 
+  interp_fm _ _ _ _ _ (FNeg f) := 
     ~ interp_fm _ _ _ _ _ f ;
-  interp_fm t_ctx tys tv _ env (FForall _ e f) := 
+  interp_fm t_ctx tys tv _ env (FForall e f) := 
     forall (x: interp_te t_ctx tys tv 0 e), 
-      interp_fm _ _ _ _ (VSnoc _ _ _ _ _ env x) f ;
-  interp_fm t_ctx tys tv _ env (FExists _ e f) := 
+      interp_fm _ _ _ _ (VSnoc env x) f ;
+  interp_fm t_ctx tys tv _ env (FExists e f) := 
     exists (x: interp_te t_ctx tys tv 0 e), 
-      interp_fm _ _ _ _ (VSnoc _ _ _ _ _ env x) f ;
+      interp_fm _ _ _ _ (VSnoc env x) f ;
 }.
 Next Obligation.
 erewrite apply_outer_eq in X.
 apply X.
 Defined.
 
-Equations interp_pfm t_ctx (tys: snoc_list Type) (tv: ty_valu t_ctx tys) (pf: poly_fm sig_sorts sig t_ctx) : Prop := {
-  interp_pfm t_ctx tys tv (PFm _ f) := 
-    interp_fm t_ctx tys tv _ (VEmp _ _ _) f;
-  interp_pfm t_ctx tys tv (PForall _ pf) := 
+Equations interp_pfm t_ctx (tys: snoc_list Type) (tv: ty_valu t_ctx tys) (pf: poly_fm (sig := sig) t_ctx) : Prop := {
+  interp_pfm t_ctx tys tv (PFm f) := 
+    interp_fm t_ctx tys tv _ VEmp f;
+  interp_pfm t_ctx tys tv (PForall pf) := 
     forall (T: Type), 
-      interp_pfm _ _ (TVSnoc _ T _ _) pf;
+      interp_pfm _ _ (TVSnoc _ T) pf;
 }.
-
 
 End PolySemantics.
 
+Arguments VEmp {_ _ _ _ _}.
+Arguments VSnoc {_ _ _ _ _ _ _} _ _.
 
-Arguments TEApp {_ _ _} _ _.
-Arguments TEVar {_ _ _} _.
-Arguments TEVAnon {_ _} _.
-Arguments TEVNamed {_ _ _} _.
-Arguments TCVHere {_}.
-
-Arguments PFm {_ _ _} _.
-Arguments PForall {_ _ _} _.
-Arguments FTrue {_ _ _ _}.
-Arguments FForall {_ _ _ _} _ _.
-Arguments FEq {_ _ _ _ _} _ _.
-Arguments TVar {_ _ _ _ _} _.
-Arguments VHere {_ _ _ _}.
-Arguments VThere {_ _ _ _ _} _.
-Arguments TFun {_ _ _ _ _ _ _ _} _ _ _.
-
-
-Section PolyDemo.
-
-Require Import Coq.Lists.List.
-
-Import ListNotations.
-
-Inductive demo_sorts : nat -> Type := 
-| sort_list : demo_sorts 1
-| sort_nat : demo_sorts 0.
-
-Notation loc_A := (TEVar (TEVAnon TCVHere)).
-
-Notation list_A := (TEApp
-  (TEVar (TEVNamed sort_list)) 
-  loc_A
-).
-
-Notation nat_ty := (TEVar (TEVNamed sort_nat)).
-
-Inductive demo_funs : 
-  forall ctx, list (ty_expr demo_sorts ctx 0) -> ty_expr demo_sorts ctx 0 -> Type := 
-| demo_app : demo_funs 1 [list_A; list_A] list_A (* forall A, list A -> list A -> list A*)
-| demo_len : demo_funs 1 [list_A] nat_ty (* forall A, list A -> nat *)
-| demo_add : demo_funs 0 [nat_ty; nat_ty] nat_ty (* nat -> nat -> nat *)
-| demo_zero : demo_funs 0 [] nat_ty
-.
-
-Inductive demo_rels : 
-  forall ctx, list (ty_expr demo_sorts ctx 0) -> Type := .
-
-Definition demo_sig : signature demo_sorts := {|
-  sig_funs := demo_funs;
-  sig_rels := demo_rels;
-|}.
-
-Definition interp_demo_sorts : forall n, demo_sorts n -> arity_ftor n := fun n srt => 
-  match srt with 
-  | sort_list => list
-  | sort_nat => nat
-  end.
-
-Equations 
-  interp_demo_funs t_ctx ctx args ret (fn: demo_funs t_ctx args ret) tv (hargs: HList.t (interp_te demo_sorts interp_demo_sorts t_ctx ctx tv 0) args) : 
-  interp_te demo_sorts interp_demo_sorts t_ctx ctx tv 0 ret := {
-  interp_demo_funs _ _ _ _ demo_app _ (l ::: r ::: _) := List.app l r; 
-  interp_demo_funs _ _ _ _ demo_len _ (x ::: _) := List.length x; 
-  interp_demo_funs _ _ _ _ demo_add _ (l ::: r ::: _) := l + r; 
-  interp_demo_funs _ _ _ _ demo_zero _ _ := 0; 
-}.
-
-Definition interp_demo_rels t_ctx ctx args (fn: demo_rels t_ctx args) tv (hargs: HList.t (interp_te demo_sorts interp_demo_sorts t_ctx ctx tv 0) args) : Prop := 
-  match fn with end.
-
-Program Definition demo_model : interp_sig demo_sorts interp_demo_sorts demo_sig := {| 
-  interp_funs := interp_demo_funs;
-  interp_rels := interp_demo_rels;
-|}.
-
-
-
-
-Notation t_xs := (TVar (VThere VHere)).
-Notation t_ys := (TVar VHere).
-
-Notation t_app ty_args args := (TFun (sig := demo_sig) demo_app ty_args args).
-Notation t_len ty_args args := (TFun (sig := demo_sig) demo_len ty_args args).
-Notation t_add args := (TFun (sig := demo_sig) demo_add TVEmp args).
-Notation t_zero := (TFun (sig := demo_sig) demo_zero TVEmp hnil).
-
-Program Definition app_len_pf_syntax: 
-  poly_fm demo_sorts demo_sig 0 :=  PForall (PFm (
-    FForall list_A (FForall list_A (
-      FEq 
-        (t_len _ ((t_app _ (t_xs ::: t_ys ::: hnil)) ::: hnil))
-        (t_add ((t_len (TVSnoc _ loc_A _ TVEmp) (t_xs ::: hnil)) ::: (t_len _ (t_ys ::: hnil)) ::: hnil))
-    ))
-  )).
-
-Example app_len_pf: 
-  interp_pfm demo_sorts interp_demo_sorts demo_sig demo_model 0 SLNil TVEmp app_len_pf_syntax.
-Proof.
-  (* this short proof works as well: *)
-  (* 
-  vm_compute.
-  intros.
-  eapply List.app_length. 
-  *)
-  unfold app_len_pf_syntax.
-  autorewrite with interp_pfm.
-  unfold interp_pfm_obligations_obligation_1, interp_pfm_obligations_obligation_2.
-  intros.
-  autorewrite with interp_pfm.
-  autorewrite with interp_fm.
-  intros.
-  vm_compute in x.
-  autorewrite with interp_fm.
-  intros.
-  vm_compute in x0.
-  set (t := apply_ty_args _ _ _ _ _ _ _).
-  vm_compute in t.
-  subst t.
-  autorewrite with interp_fm.
-  unfold interp_fm_obligations_obligation_1, interp_fm_obligations_obligation_2, interp_fm_obligations_obligation_3, interp_fm_obligations_obligation_4.
-  set (t := apply_ty_args _ _ _ _ _ _ _);
-  vm_compute in t;
-  subst t.
-
-  set (l := interp_tm _ _ _ _ _ _ _ _ _ _ _).
-  set (r := interp_tm _ _ _ _ _ _ _ _ _ _ _).
-  vm_compute in l.
-  vm_compute in r.
-  eapply List.app_length.
-Qed.
-
-(* Print Assumptions app_len_pf.  *)
-
-End PolyDemo.
-
-Section GenericTheory.
-
-Variable generic_inner_sorts: nat -> Type.
-
-Inductive generic_sorts: nat -> Type :=
-| generic_arrow : generic_sorts 2
-| generic_inner: forall n, generic_inner_sorts n -> generic_sorts n.
-
-Notation loc_A := (TEVar (TEVAnon TCVHere)).
-Notation loc_B := (TEVar (TEVAnon (TCVThere _ TCVHere))).
-
-Notation arrow_A_B := (TEApp (TEApp (TEVar (TEVNamed generic_arrow)) loc_A) loc_B).
-
-Import ListNotations.
-
-Inductive generic_funs:
-  forall ctx, list (ty_expr generic_sorts ctx 0) -> ty_expr generic_sorts ctx 0 -> Type :=
-| generic_eval : generic_funs 2 [arrow_A_B; loc_A] loc_B (* forall A B, arrow A B -> A -> B*)
-.
-
-Inductive generic_rels:
-  forall ctx, list (ty_expr generic_sorts ctx 0) -> Type := .
-
-Definition generic_sig: signature generic_sorts := {|
-  sig_funs := generic_funs;
-  sig_rels := generic_rels;
-|}.
-
-Variable interp_generic_inner_sorts : forall n (sort: generic_inner_sorts n), arity_ftor n.
-
-Equations interp_generic_sorts n (sort: generic_sorts n) : arity_ftor n := {
-    interp_generic_sorts _ generic_arrow := fun A B => A -> B;
-    interp_generic_sorts n (generic_inner n inner_sort) := interp_generic_inner_sorts n inner_sort
-}.
-
-Equations
-  interp_generic_funs t_ctx ctx args ret (fn: generic_funs t_ctx args ret)
-    tv (hargs: HList.t (interp_te generic_sorts interp_generic_sorts t_ctx ctx tv 0) args) :
-  interp_te generic_sorts interp_generic_sorts t_ctx ctx tv 0 ret := {
-  interp_generic_funs _ _ _ _ generic_eval _ (f ::: arg ::: _) := f arg;
-}.
-
-Definition interp_generic_rels t_ctx ctx args (rel: generic_rels t_ctx args) tv (hargs: HList.t (interp_te generic_sorts interp_generic_sorts t_ctx ctx tv 0) args) : Prop :=
-  match rel with end.
-
-Program Definition generic_model : interp_sig generic_sorts interp_generic_sorts generic_sig := {|
-  interp_funs := interp_generic_funs;
-  interp_rels := interp_generic_rels;
-|}.
-
-End GenericTheory.
-
-Section GenericDemo.
-
-Inductive generic_inner_sorts : nat -> Type :=
-| inner_sort_list : generic_inner_sorts 1
-| inner_sort_nat : generic_inner_sorts 0.
-
-Notation te_arrow A B := (TEApp (TEApp (TEVar (TEVNamed (generic_arrow generic_inner_sorts))) A) B).
-Notation loc_A := (TEVar (TEVAnon TCVHere)).
-Notation list_A := (TEApp (TEVar (TEVNamed (generic_inner _ _ inner_sort_list))) loc_A).
-Notation nat' := (TEVar (TEVNamed (generic_inner _ _ inner_sort_nat))).
-Notation len_A := (te_arrow list_A nat').
-Notation app_A := (te_arrow list_A (te_arrow list_A list_A)).
-Notation cons_A := (te_arrow loc_A (te_arrow list_A list_A)).
-Notation add' := (te_arrow nat' (te_arrow nat' nat')).
-Notation t_eval ty_args args := (TFun (sig := generic_sig generic_inner_sorts) (generic_eval _) ty_args args).
-Notation t_len_A arg := (t_eval (TVSnoc _ list_A _ (TVSnoc _ nat' _ TVEmp))
-                                 (TVar (VThere (VThere (VThere (VThere (VThere VHere))))) ::: arg ::: hnil)).
-Notation t_app_A x y := (t_eval (TVSnoc _ list_A _ (TVSnoc _ list_A _ TVEmp))
-                              (t_eval (TVSnoc _ list_A _ (TVSnoc _ (te_arrow list_A list_A) _ TVEmp))
-                              (TVar (VThere (VThere (VThere (VThere (VThere VHere))))) ::: x ::: hnil) ::: y ::: hnil)).
-Notation t_app_A' x y := (t_eval (TVSnoc _ list_A _ (TVSnoc _ list_A _ TVEmp))
-                              (t_eval (TVSnoc _ list_A _ (TVSnoc _ (te_arrow list_A list_A) _ TVEmp))
-                              (TVar (VThere (VThere (VThere (VThere VHere)))) ::: x ::: hnil) ::: y ::: hnil)).
-Notation t_cons_A a x := (t_eval (TVSnoc _ list_A _ (TVSnoc _ list_A _ TVEmp))
-                              (t_eval (TVSnoc _ loc_A _ (TVSnoc _ (te_arrow list_A list_A) _ TVEmp))
-                              (TVar (VThere (VThere (VThere (VThere VHere)))) ::: a ::: hnil) ::: x ::: hnil)).
-Notation t_add' x y := (t_eval (TVSnoc _ nat' _ (TVSnoc _ nat' _ TVEmp))
-                              (t_eval (TVSnoc _ nat' _ (TVSnoc _ (te_arrow nat' nat') _ TVEmp))
-                              (TVar (VThere (VThere VHere)) ::: x ::: hnil) ::: y ::: hnil)).
-
-Check FForall add' (
-    FImpl _ _ _ _
-        (
-        FForall loc_A (
-        FForall list_A (
-        FForall list_A (
-          FEq
-            (t_app_A (t_cons_A (TVar (VThere (VThere VHere))) (TVar (VThere VHere))) (TVar VHere))
-            (t_cons_A (TVar (VThere (VThere VHere))) (t_app_A (TVar (VThere VHere)) (TVar VHere)))
-        ))))
-        (FForall list_A (
-        FForall list_A (
-          FEq
-            (t_len_A (t_app_A' (TVar VHere) (TVar (VThere VHere))))
-            (t_add' (t_len_A (TVar VHere)) (t_len_A (TVar (VThere VHere))))
-        )))
-    ).
-
-Definition generic_test:
-  poly_fm (generic_sorts generic_inner_sorts) (generic_sig generic_inner_sorts) 0 :=
-  PForall (PFm (
-    FForall len_A (
-    FForall app_A (
-    FForall cons_A (
-    FForall add' (
-    FImpl _ _ _ _
-        (
-        FForall loc_A (
-    FForall list_A (
-    FForall list_A (
-      FEq
-            (t_app_A (t_cons_A (TVar (VThere (VThere VHere))) (TVar (VThere VHere))) (TVar VHere))
-            (t_cons_A (TVar (VThere (VThere VHere))) (t_app_A (TVar (VThere VHere)) (TVar VHere)))
-        ))))
-        (FForall list_A (
-        FForall list_A (
-          FEq
-            (t_len_A (t_app_A' (TVar VHere) (TVar (VThere VHere))))
-            (t_add' (t_len_A (TVar VHere)) (t_len_A (TVar (VThere VHere))))
-        )))
-    )))
-  ))).
-
-Definition interp_generic_sorts_inner : forall n, generic_inner_sorts n -> arity_ftor n := fun n srt =>
-  match srt with
-  | inner_sort_list => list
-  | inner_sort_nat => nat
-  end.
-
-Example app_len_generic:
-    interp_pfm (generic_sorts generic_inner_sorts) (interp_generic_sorts generic_inner_sorts interp_generic_sorts_inner) (generic_sig generic_inner_sorts) (generic_model generic_inner_sorts interp_generic_sorts_inner) 0 SLNil TVEmp generic_test.
-Proof.
-  vm_compute.
-Abort.
-
-End GenericDemo.
-
-Section ParametrizedTheory.
-
-Open Scope type_scope.
-
-Variable parametrized_inner_sorts: nat -> Type.
-
-Inductive parametrized_sorts: nat -> Type :=
-| parametrized_arrow : parametrized_sorts 2
-| parametrized_inner: forall n, parametrized_inner_sorts n -> parametrized_sorts n.
-
-Definition parametrized_manifest :=
-    list {ctx & list (ty_expr parametrized_sorts ctx 0) *
-                ty_expr parametrized_sorts ctx 0}.
-
-Inductive parametrized_funs_open:
-    parametrized_manifest ->
-    forall ctx,
-    list (ty_expr parametrized_sorts ctx 0) ->
-    ty_expr parametrized_sorts ctx 0 ->
-    Type
-:=
-| PFunHere:
-    forall ctx
-           tail
-           (args: list (ty_expr parametrized_sorts ctx 0))
-           (ret: ty_expr parametrized_sorts ctx 0),
-        parametrized_funs_open (existT _ ctx (args, ret) :: tail) ctx args ret
-| PFunThere:
-    forall ctx
-           head
-           tail
-           (args: list (ty_expr parametrized_sorts ctx 0))
-           (ret: ty_expr parametrized_sorts ctx 0),
-        parametrized_funs_open tail ctx args ret ->
-        parametrized_funs_open (head :: tail) ctx args ret
-.
-
-Variable parametrized_inner_funcs: parametrized_manifest.
-
-Definition parametrized_funs := parametrized_funs_open parametrized_inner_funcs.
-
-Inductive parametrized_rels:
-  forall ctx, list (ty_expr parametrized_sorts ctx 0) -> Type := .
-
-Definition parametrized_sig: signature parametrized_sorts := {|
-  sig_funs := parametrized_funs;
-  sig_rels := parametrized_rels;
-|}.
-
-Variable interp_parametrized_inner_sorts : forall n (sort: parametrized_inner_sorts n), arity_ftor n.
-
-Equations interp_parametrized_sorts n (sort: parametrized_sorts n) : arity_ftor n := {
-    interp_parametrized_sorts _ parametrized_arrow := fun A B => A -> B;
-    interp_parametrized_sorts n (parametrized_inner n inner_sort) := interp_parametrized_inner_sorts n inner_sort
-}.
-
-End ParametrizedTheory.
