tests/PolyDemos.v
@@ -1,0 +1,521 @@
+From Equations Require Import Equations.
+Require Import Coq.Program.Equality.
+Require Import MirrorSolve.HLists.
+
+Require Import MirrorSolve.PolyFirstOrder.
+
+Import HListNotations.
+
+Set Universe Polymorphism.
+
+
+
+Section PolyDemo.
+
+Require Import Coq.Lists.List.
+
+Import ListNotations.
+
+Inductive demo_sorts : nat -> Type := 
+| sort_list : demo_sorts 1
+| sort_nat : demo_sorts 0.
+
+Notation loc_A := (TEVar (TEVAnon TCVHere)).
+
+Notation list_A := (TEApp
+  (TEVar (TEVNamed sort_list)) 
+  loc_A
+).
+
+Notation nat_ty := (TEVar (TEVNamed sort_nat)).
+
+Inductive demo_funs : 
+  forall ctx, list (ty_expr demo_sorts ctx 0) -> ty_expr demo_sorts ctx 0 -> Type := 
+| demo_app : demo_funs 1 [list_A; list_A] list_A (* forall A, list A -> list A -> list A*)
+| demo_len : demo_funs 1 [list_A] nat_ty (* forall A, list A -> nat *)
+| demo_add : demo_funs 0 [nat_ty; nat_ty] nat_ty (* nat -> nat -> nat *)
+| demo_zero : demo_funs 0 [] nat_ty
+.
+
+Inductive demo_rels : 
+  forall ctx, list (ty_expr demo_sorts ctx 0) -> Type := .
+
+Definition demo_sig : signature demo_sorts := {|
+  sig_funs := demo_funs;
+  sig_rels := demo_rels;
+|}.
+
+Definition interp_demo_sorts : forall n, demo_sorts n -> arity_ftor n := fun n srt => 
+  match srt with 
+  | sort_list => list
+  | sort_nat => nat
+  end.
+
+Equations 
+  interp_demo_funs t_ctx ctx args ret (fn: demo_funs t_ctx args ret) tv (hargs: HList.t (interp_te demo_sorts interp_demo_sorts t_ctx ctx tv 0) args) : 
+  interp_te demo_sorts interp_demo_sorts t_ctx ctx tv 0 ret := {
+  interp_demo_funs _ _ _ _ demo_app _ (l ::: r ::: _) := List.app l r; 
+  interp_demo_funs _ _ _ _ demo_len _ (x ::: _) := List.length x; 
+  interp_demo_funs _ _ _ _ demo_add _ (l ::: r ::: _) := l + r; 
+  interp_demo_funs _ _ _ _ demo_zero _ _ := 0; 
+}.
+
+Definition interp_demo_rels t_ctx ctx args (fn: demo_rels t_ctx args) tv (hargs: HList.t (interp_te demo_sorts interp_demo_sorts t_ctx ctx tv 0) args) : Prop := 
+  match fn with end.
+
+Program Definition demo_model : interp_sig demo_sorts interp_demo_sorts demo_sig := {| 
+  interp_funs := interp_demo_funs;
+  interp_rels := interp_demo_rels;
+|}.
+
+
+
+
+Notation t_xs := (TVar (VThere VHere)).
+Notation t_ys := (TVar VHere).
+
+Notation t_app ty_args args := (TFun (sig := demo_sig) demo_app ty_args args).
+Notation t_len ty_args args := (TFun (sig := demo_sig) demo_len ty_args args).
+Notation t_add args := (TFun (sig := demo_sig) demo_add TVEmp args).
+Notation t_zero := (TFun (sig := demo_sig) demo_zero TVEmp hnil).
+
+Program Definition app_len_pf_syntax: 
+  poly_fm demo_sorts demo_sig 0 :=  PForall (PFm (
+    FForall list_A (FForall list_A (
+      FEq 
+        (t_len _ ((t_app _ (t_xs ::: t_ys ::: hnil)) ::: hnil))
+        (t_add ((t_len (TVSnoc _ loc_A _ TVEmp) (t_xs ::: hnil)) ::: (t_len _ (t_ys ::: hnil)) ::: hnil))
+    ))
+  )).
+
+Example app_len_pf: 
+  interp_pfm demo_sorts interp_demo_sorts demo_sig demo_model 0 SLNil TVEmp app_len_pf_syntax.
+Proof.
+  (* this short proof works as well: *)
+  (* 
+  vm_compute.
+  intros.
+  eapply List.app_length. 
+  *)
+  unfold app_len_pf_syntax.
+  autorewrite with interp_pfm.
+  unfold interp_pfm_obligations_obligation_1, interp_pfm_obligations_obligation_2.
+  intros.
+  autorewrite with interp_pfm.
+  autorewrite with interp_fm.
+  intros.
+  vm_compute in x.
+  autorewrite with interp_fm.
+  intros.
+  vm_compute in x0.
+  set (t := apply_ty_args _ _ _ _ _ _ _).
+  vm_compute in t.
+  subst t.
+  autorewrite with interp_fm.
+  unfold interp_fm_obligations_obligation_1, interp_fm_obligations_obligation_2, interp_fm_obligations_obligation_3, interp_fm_obligations_obligation_4.
+  set (t := apply_ty_args _ _ _ _ _ _ _);
+  vm_compute in t;
+  subst t.
+
+  set (l := interp_tm _ _ _ _ _ _ _ _ _ _ _).
+  set (r := interp_tm _ _ _ _ _ _ _ _ _ _ _).
+  vm_compute in l.
+  vm_compute in r.
+  eapply List.app_length.
+Qed.
+
+(* Print Assumptions app_len_pf.  *)
+
+End PolyDemo.
+
+Section GenericTheory.
+
+Variable generic_inner_sorts: nat -> Type.
+
+Inductive generic_sorts: nat -> Type :=
+| generic_arrow : generic_sorts 2
+| generic_inner: forall n, generic_inner_sorts n -> generic_sorts n.
+
+Notation loc_A := (TEVar (TEVAnon TCVHere)).
+Notation loc_B := (TEVar (TEVAnon (TCVThere _ TCVHere))).
+
+Notation arrow_A_B := (TEApp (TEApp (TEVar (TEVNamed generic_arrow)) loc_A) loc_B).
+
+Import ListNotations.
+
+Inductive generic_funs:
+  forall ctx, list (ty_expr generic_sorts ctx 0) -> ty_expr generic_sorts ctx 0 -> Type :=
+| generic_eval : generic_funs 2 [arrow_A_B; loc_A] loc_B (* forall A B, arrow A B -> A -> B*)
+.
+
+Inductive generic_rels:
+  forall ctx, list (ty_expr generic_sorts ctx 0) -> Type := .
+
+Definition generic_sig: signature generic_sorts := {|
+  sig_funs := generic_funs;
+  sig_rels := generic_rels;
+|}.
+
+Variable interp_generic_inner_sorts : forall n (sort: generic_inner_sorts n), arity_ftor n.
+
+Equations interp_generic_sorts n (sort: generic_sorts n) : arity_ftor n := {
+    interp_generic_sorts _ generic_arrow := fun A B => A -> B;
+    interp_generic_sorts n (generic_inner n inner_sort) := interp_generic_inner_sorts n inner_sort
+}.
+
+Equations
+  interp_generic_funs t_ctx ctx args ret (fn: generic_funs t_ctx args ret)
+    tv (hargs: HList.t (interp_te generic_sorts interp_generic_sorts t_ctx ctx tv 0) args) :
+  interp_te generic_sorts interp_generic_sorts t_ctx ctx tv 0 ret := {
+  interp_generic_funs _ _ _ _ generic_eval _ (f ::: arg ::: _) := f arg;
+}.
+
+Definition interp_generic_rels t_ctx ctx args (rel: generic_rels t_ctx args) tv (hargs: HList.t (interp_te generic_sorts interp_generic_sorts t_ctx ctx tv 0) args) : Prop :=
+  match rel with end.
+
+Program Definition generic_model : interp_sig generic_sorts interp_generic_sorts generic_sig := {|
+  interp_funs := interp_generic_funs;
+  interp_rels := interp_generic_rels;
+|}.
+
+End GenericTheory.
+
+Section GenericDemo.
+
+Inductive generic_inner_sorts : nat -> Type :=
+| inner_sort_list : generic_inner_sorts 1
+| inner_sort_nat : generic_inner_sorts 0.
+
+Notation te_arrow A B := (TEApp (TEApp (TEVar (TEVNamed (generic_arrow generic_inner_sorts))) A) B).
+Notation loc_A := (TEVar (TEVAnon TCVHere)).
+Notation list_A := (TEApp (TEVar (TEVNamed (generic_inner _ _ inner_sort_list))) loc_A).
+Notation nat' := (TEVar (TEVNamed (generic_inner _ _ inner_sort_nat))).
+Notation len_A := (te_arrow list_A nat').
+Notation app_A := (te_arrow list_A (te_arrow list_A list_A)).
+Notation cons_A := (te_arrow loc_A (te_arrow list_A list_A)).
+Notation add' := (te_arrow nat' (te_arrow nat' nat')).
+Notation t_eval ty_args args := (TFun (sig := generic_sig generic_inner_sorts) (generic_eval _) ty_args args).
+Notation t_len_A arg := (t_eval (TVSnoc _ list_A _ (TVSnoc _ nat' _ TVEmp))
+                                 (TVar (VThere (VThere (VThere (VThere (VThere VHere))))) ::: arg ::: hnil)).
+Notation t_app_A x y := (t_eval (TVSnoc _ list_A _ (TVSnoc _ list_A _ TVEmp))
+                              (t_eval (TVSnoc _ list_A _ (TVSnoc _ (te_arrow list_A list_A) _ TVEmp))
+                              (TVar (VThere (VThere (VThere (VThere (VThere VHere))))) ::: x ::: hnil) ::: y ::: hnil)).
+Notation t_app_A' x y := (t_eval (TVSnoc _ list_A _ (TVSnoc _ list_A _ TVEmp))
+                              (t_eval (TVSnoc _ list_A _ (TVSnoc _ (te_arrow list_A list_A) _ TVEmp))
+                              (TVar (VThere (VThere (VThere (VThere VHere)))) ::: x ::: hnil) ::: y ::: hnil)).
+Notation t_cons_A a x := (t_eval (TVSnoc _ list_A _ (TVSnoc _ list_A _ TVEmp))
+                              (t_eval (TVSnoc _ loc_A _ (TVSnoc _ (te_arrow list_A list_A) _ TVEmp))
+                              (TVar (VThere (VThere (VThere (VThere VHere)))) ::: a ::: hnil) ::: x ::: hnil)).
+Notation t_add' x y := (t_eval (TVSnoc _ nat' _ (TVSnoc _ nat' _ TVEmp))
+                              (t_eval (TVSnoc _ nat' _ (TVSnoc _ (te_arrow nat' nat') _ TVEmp))
+                              (TVar (VThere (VThere VHere)) ::: x ::: hnil) ::: y ::: hnil)).
+
+Check FForall add' (
+    FImpl _ _ _ _
+        (
+        FForall loc_A (
+        FForall list_A (
+        FForall list_A (
+          FEq
+            (t_app_A (t_cons_A (TVar (VThere (VThere VHere))) (TVar (VThere VHere))) (TVar VHere))
+            (t_cons_A (TVar (VThere (VThere VHere))) (t_app_A (TVar (VThere VHere)) (TVar VHere)))
+        ))))
+        (FForall list_A (
+        FForall list_A (
+          FEq
+            (t_len_A (t_app_A' (TVar VHere) (TVar (VThere VHere))))
+            (t_add' (t_len_A (TVar VHere)) (t_len_A (TVar (VThere VHere))))
+        )))
+    ).
+
+Definition generic_test:
+  poly_fm (generic_sorts generic_inner_sorts) (generic_sig generic_inner_sorts) 0 :=
+  PForall (PFm (
+    FForall len_A (
+    FForall app_A (
+    FForall cons_A (
+    FForall add' (
+    FImpl _ _ _ _
+        (
+        FForall loc_A (
+    FForall list_A (
+    FForall list_A (
+      FEq
+            (t_app_A (t_cons_A (TVar (VThere (VThere VHere))) (TVar (VThere VHere))) (TVar VHere))
+            (t_cons_A (TVar (VThere (VThere VHere))) (t_app_A (TVar (VThere VHere)) (TVar VHere)))
+        ))))
+        (FForall list_A (
+        FForall list_A (
+          FEq
+            (t_len_A (t_app_A' (TVar VHere) (TVar (VThere VHere))))
+            (t_add' (t_len_A (TVar VHere)) (t_len_A (TVar (VThere VHere))))
+        )))
+    )))
+  ))).
+
+Definition interp_generic_sorts_inner : forall n, generic_inner_sorts n -> arity_ftor n := fun n srt =>
+  match srt with
+  | inner_sort_list => list
+  | inner_sort_nat => nat
+  end.
+
+Example app_len_generic:
+    interp_pfm (generic_sorts generic_inner_sorts) (interp_generic_sorts generic_inner_sorts interp_generic_sorts_inner) (generic_sig generic_inner_sorts) (generic_model generic_inner_sorts interp_generic_sorts_inner) 0 SLNil TVEmp generic_test.
+Proof.
+  vm_compute.
+Abort.
+
+End GenericDemo.
+
+Section ParametrizedTheory.
+
+Open Scope type_scope.
+
+Variable parametrized_inner_sorts: nat -> Type.
+
+Inductive parametrized_sorts: nat -> Type :=
+| parametrized_arrow : parametrized_sorts 2
+| parametrized_inner: forall n, parametrized_inner_sorts n -> parametrized_sorts n.
+
+Definition parametrized_manifest :=
+    list {ctx & list (ty_expr parametrized_sorts ctx 0) *
+                ty_expr parametrized_sorts ctx 0}.
+
+Inductive parametrized_funs_open:
+    parametrized_manifest ->
+    forall ctx,
+    list (ty_expr parametrized_sorts ctx 0) ->
+    ty_expr parametrized_sorts ctx 0 ->
+    Type
+:=
+| PFunHere:
+    forall ctx
+           tail
+           (args: list (ty_expr parametrized_sorts ctx 0))
+           (ret: ty_expr parametrized_sorts ctx 0),
+        parametrized_funs_open (existT _ ctx (args, ret) :: tail) ctx args ret
+| PFunThere:
+    forall ctx
+           head
+           tail
+           (args: list (ty_expr parametrized_sorts ctx 0))
+           (ret: ty_expr parametrized_sorts ctx 0),
+        parametrized_funs_open tail ctx args ret ->
+        parametrized_funs_open (head :: tail) ctx args ret
+.
+
+Variable parametrized_inner_funcs: parametrized_manifest.
+
+Definition parametrized_funs := parametrized_funs_open parametrized_inner_funcs.
+
+Inductive parametrized_rels:
+  forall ctx, list (ty_expr parametrized_sorts ctx 0) -> Type := .
+
+Definition parametrized_sig: signature parametrized_sorts := {|
+  sig_funs := parametrized_funs;
+  sig_rels := parametrized_rels;
+|}.
+
+Variable interp_parametrized_inner_sorts : forall n (sort: parametrized_inner_sorts n), arity_ftor n.
+
+Equations interp_parametrized_sorts n (sort: parametrized_sorts n) : arity_ftor n := {
+    interp_parametrized_sorts _ parametrized_arrow := fun A B => A -> B;
+    interp_parametrized_sorts n (parametrized_inner n inner_sort) := interp_parametrized_inner_sorts n inner_sort
+}.
+
+End ParametrizedTheory.
+
+
+Section ConstantTypesAbstractedTheory.
+
+Variable inner_sorts: nat -> Type.
+
+Variable constant_sorts: Type.
+
+Inductive abstract_sorts: nat -> Type :=
+| abstract_constant : constant_sorts -> abstract_sorts 0
+| abstract_inner_sort: forall n, inner_sorts n -> abstract_sorts n.
+
+Variable inner_funs:
+  forall ctx,
+    list (ty_expr inner_sorts ctx 0) ->
+    ty_expr inner_sorts ctx 0 ->
+    Type
+.
+
+Equations abstract_ty_expr_var
+  {n ctx}
+  (var: ty_expr_var inner_sorts ctx n)
+:
+  ty_expr_var abstract_sorts ctx n
+:= {
+  abstract_ty_expr_var (TEVAnon var) :=
+    TEVAnon var;
+  abstract_ty_expr_var (TEVNamed name) :=
+    TEVNamed (abstract_inner_sort _ name);
+}.
+
+Equations abstract_ty_expr
+  {n ctx}
+  (var: ty_expr inner_sorts ctx n)
+:
+  ty_expr abstract_sorts ctx n
+:= {
+  abstract_ty_expr (TEVar var) :=
+    TEVar (abstract_ty_expr_var var);
+  abstract_ty_expr (TEApp func arg) :=
+    TEApp (abstract_ty_expr func)
+          (abstract_ty_expr arg);
+}.
+
+Inductive abstract_funs:
+  forall ctx,
+    list (ty_expr abstract_sorts ctx 0) ->
+    ty_expr abstract_sorts ctx 0 ->
+    Type
+:=
+| abstract_inner_fun:
+    forall ctx args ret,
+      inner_funs ctx args ret ->
+      abstract_funs ctx (map abstract_ty_expr args)
+                        (abstract_ty_expr ret)
+.
+
+Variable inner_rels:
+  forall ctx,
+    list (ty_expr inner_sorts ctx 0) ->
+    Type
+.
+
+Inductive abstract_rels:
+  forall ctx,
+    list (ty_expr abstract_sorts ctx 0) ->
+    Type
+:=
+| abstract_inner_rel:
+    forall ctx args,
+      inner_rels ctx args ->
+      abstract_rels ctx (map abstract_ty_expr args)
+.
+
+Definition abstract_sig: signature abstract_sorts := {|
+  sig_funs := abstract_funs;
+  sig_rels := abstract_rels;
+|}.
+
+Variable interp_inner_sorts: forall n (sort: inner_sorts n), arity_ftor n.
+Variable interp_constants: constant_sorts -> Type.
+
+Equations interp_abstract_sorts n (sort: abstract_sorts n) : arity_ftor n := {
+  interp_abstract_sorts _ (abstract_inner_sort n inner_sort) := interp_inner_sorts n inner_sort;
+  interp_abstract_sorts _ (abstract_constant constant) := interp_constants constant;
+}.
+
+Variable interp_inner_funs:
+  forall t_ctx ctx args ret (fn: inner_funs t_ctx args ret) tv
+    (hargs: HList.t (interp_te inner_sorts interp_inner_sorts t_ctx ctx tv 0) args),
+    interp_te inner_sorts interp_inner_sorts t_ctx ctx tv 0 ret
+.
+
+Equations concretize_interp_te_var 
+  t_ctx ctx tv te_var 
+  (val: interp_te_var abstract_sorts interp_abstract_sorts ctx t_ctx tv 0 (abstract_ty_expr_var te_var)) 
+: interp_te_var inner_sorts interp_inner_sorts ctx t_ctx tv 0 te_var := {
+  concretize_interp_te_var _ _ _ (TEVAnon _) val := val;
+  concretize_interp_te_var _ _ _ (TEVNamed _) val := val;
+}.
+
+Definition concretize_interp_te t_ctx ctx tv n ty_expr: interp_te abstract_sorts interp_abstract_sorts t_ctx ctx tv n (abstract_ty_expr ty_expr) = interp_te inner_sorts interp_inner_sorts t_ctx ctx tv n ty_expr.
+Proof.
+  dependent induction ty_expr; autorewrite with abstract_ty_expr.
+  - autorewrite with abstract_ty_expr.
+    dependent destruction t; now autorewrite with abstract_ty_expr_var.
+  - autorewrite with interp_te; simpl.
+    now rewrite IHty_expr1, IHty_expr2.
+Defined.
+
+Definition concretize_interp_te' t_ctx ctx tv ty_expr: interp_te abstract_sorts interp_abstract_sorts t_ctx ctx tv 0 (abstract_ty_expr ty_expr) -> interp_te inner_sorts interp_inner_sorts t_ctx ctx tv 0 ty_expr.
+Proof.
+  intro.
+  now rewrite concretize_interp_te in X.
+Defined.
+
+
+(* 
+  Synthesize the term by swapping the map in the params HList to get an HList over the
+  original arguments, use the equality of the interpretations, use HList map to 
+  convert the interpreted abstract arguments back to their original values.
+*)
+Local Obligation Tactic := intros.
+Equations
+  interp_abstract_funs 
+    t_ctx ctx args ret 
+    (fn: abstract_funs t_ctx args ret) tv 
+    (hargs: HList.t (interp_te abstract_sorts interp_abstract_sorts t_ctx ctx tv 0) args) 
+: interp_te abstract_sorts interp_abstract_sorts t_ctx ctx tv 0 ret := {
+  interp_abstract_funs _ _ _ _ (abstract_inner_fun _ _ _ inner_fun) _ args := 
+    let swapped := HList.map_swap _ _ args in 
+      _;
+}.
+Next Obligation.
+erewrite concretize_interp_te.
+eapply interp_inner_funs; eauto.
+eapply HList.map.
+2: eapply swapped.
+intros.
+simpl in X.
+eapply concretize_interp_te'.
+exact X.
+Defined.
+
+Variable interp_inner_rels:
+  forall t_ctx ctx args (fn: inner_rels t_ctx args) tv
+    (hargs: HList.t (interp_te inner_sorts interp_inner_sorts t_ctx ctx tv 0) args),
+    Prop
+.
+
+Equations
+  interp_abstract_rels 
+    t_ctx ctx args 
+    (fn: abstract_rels t_ctx args) tv 
+    (hargs: HList.t (interp_te abstract_sorts interp_abstract_sorts t_ctx ctx tv 0) args) 
+: Prop := {
+  interp_abstract_rels _ _ _ (abstract_inner_rel _ _ inner_rel) _ args := 
+    let swapped := HList.map_swap _ _ args in 
+      _;
+}.
+Next Obligation.
+eapply interp_inner_rels; eauto.
+eapply HList.map.
+2: eapply swapped.
+intros.
+simpl in X.
+eapply concretize_interp_te'.
+exact X.
+Defined.
+
+
+Program Definition abstract_model : interp_sig abstract_sorts interp_abstract_sorts abstract_sig := {|
+  interp_funs := interp_abstract_funs;
+  interp_rels := interp_abstract_rels;
+|}.
+
+Definition inner_sig : signature inner_sorts := {| 
+  sig_funs := inner_funs;
+  sig_rels := inner_rels;
+|}.
+
+Fixpoint get_poly_context {ctx} (pfm: poly_fm inner_sorts inner_sig ctx) : ty_ctx :=
+  match pfm with 
+  | PFm _ => ctx
+  | PForall inner => 
+    get_poly_context inner
+  end.
+
+Fixpoint get_poly_fm {ctx} (pfm: poly_fm inner_sorts inner_sig ctx) : fm inner_sorts inner_sig (get_poly_context pfm) SLNil := 
+  match pfm with 
+  | PFm f => f
+  | PForall inner => get_poly_fm inner
+  end.
+
+(* TODO: walk the term and rewrite function and relation symbols; prove the two are bi-satisfactory *)
